theories/Languages/Lustre.v
@@ -172,3 +172,278 @@ Inductive sem_exp: history -> exp -> value -> Prop :=
       sem_exp h e1 v1 ->
       sem_exp h e2 v2 ->
       sem_exp h (EBinop op e1 e2) (VBinop op v1 v2).
+
+
+(** ** Properties *)
+
+Fixpoint eval_exp (e: exp) (h: history): option value :=
+  match e with
+    | EConst c => Some (VConst c)
+    | EInput b => Some (VInput b)
+    | EVar (name, typ) => Dict.find name h
+    | EBinop op e1 e2 => match eval_exp e1 h, eval_exp e2 h with
+      | Some v1, Some v2 => Some (VBinop op v1 v2)
+      | _, _ => None
+    end
+  end.
+
+Definition is_evaluable (e: exp) (h: history): Prop :=
+  exists v: value, eval_exp e h = Some v.
+
+
+(** ** Lemmas *)
+
+Lemma var_of_exp_aux_non_empty (e: exp) (l: list ident):
+  l <> [] -> var_of_exp_aux e l <> [].
+Proof.
+  intros Hl He.
+  revert l Hl He.
+  induction e as [ | | v | op e1 IHe1 e2 IHe2 ]; intros l Hl He.
+  - simpl in He.
+    contradiction.
+  - simpl in He.
+    apply Hl.
+    assumption.
+  - destruct v.
+    simpl in He.
+    discriminate.
+  - simpl in He.
+    apply IHe1 with (l := var_of_exp_aux e2 l).
+    + intros He2.
+      apply IHe2 with (l := l); assumption.
+    + assumption.
+Qed.
+
+Lemma var_of_exp_aux_empty (e: exp) (l: list ident):
+  var_of_exp_aux e l = [] -> l = [].
+Proof.
+  revert l.
+  induction e as [ | | v | op e1 IHe1 e2 IHe2 ]; intros l H.
+  - simpl in H.
+    assumption.
+  - assumption.
+  - destruct v.
+    simpl in H.
+    discriminate.
+  - simpl in H.
+    apply IHe2.
+    apply IHe1.
+    assumption.
+Qed.
+
+Lemma var_of_exp_aux_incl (e: exp) (l1 l2: list ident):
+  incl l1 l2 -> incl (var_of_exp_aux e l1) (var_of_exp_aux e l2).
+Proof.
+  intros H x Hx.
+  revert l1 l2 x H Hx.
+  induction e; intros l1 l2 x H Hx; simpl in *.
+  - apply H.
+    assumption.
+  - apply H.
+    assumption.
+  - destruct b as [ i t ].
+    destruct Hx as [ Hx | Hx ].
+    + left.
+      assumption.
+    + right.
+      apply H.
+      assumption.
+  - apply IHe1 with (l1 := var_of_exp_aux e2 l1); [ | assumption ].
+    intros y Hy.
+    apply IHe2 with (l1 := l1); assumption.
+Qed.
+
+Lemma var_of_exp_aux_in_exp (e: exp) (l: list ident) (x: ident):
+  In x (var_of_exp e) -> In x (var_of_exp_aux e l).
+Proof.
+  apply var_of_exp_aux_incl with (l1 := []).
+  intros a Hin.
+  destruct Hin.
+Qed.
+
+Lemma var_of_exp_aux_in_acc (e: exp) (l: list ident) (x: ident):
+  In x l -> In x (var_of_exp_aux e l).
+Proof.
+  revert l.
+  induction e; intros l H.
+  - assumption.
+  - assumption.
+  - destruct b.
+    right.
+    assumption.
+  - simpl.
+    apply IHe1.
+    apply IHe2.
+    assumption.
+Qed.
+
+Lemma var_of_exp_aux_eq (e: exp) (l: list ident):
+  var_of_exp_aux e l = var_of_exp e ++ l.
+Proof.
+  revert l.
+  induction e as [ c | | (v, t) | op e1 IH1 e2 IH2 ]; intros l; [ reflexivity.. | ].
+  unfold var_of_exp.
+  simpl.
+  rewrite IH1.
+  rewrite IH1.
+  rewrite IH2.
+  rewrite app_assoc.
+  reflexivity.
+Qed.
+
+Lemma var_of_exp_not_in_binop (exp1 exp2: exp) (x: ident) (b: binop):
+  ~ In x (var_of_exp (EBinop b exp1 exp2)) ->
+  ~ In x (var_of_exp exp1) /\ ~ In x (var_of_exp exp2).
+Proof.
+  intros Hnin.
+  split.
+  - intros Hin1.
+    apply Hnin.
+    unfold var_of_exp.
+    simpl.
+    apply var_of_exp_aux_in_exp.
+    assumption.
+  - intros Hin1.
+    apply Hnin.
+    unfold var_of_exp.
+    simpl.
+    apply var_of_exp_aux_in_acc.
+    assumption.
+Qed.
+
+Lemma var_of_exp_binop_empty (exp1 exp2: exp) (b: binop):
+  var_of_exp (EBinop b exp1 exp2) = [] ->
+  var_of_exp exp1 = [] /\ var_of_exp exp2 = [].
+Proof.
+  intros H.
+  split.
+  - unfold var_of_exp in *.
+    simpl in H.
+    apply var_of_exp_aux_empty in H as H2.
+    rewrite H2 in H.
+    assumption.
+  - unfold var_of_exp in *.
+    simpl in H.
+    apply var_of_exp_aux_empty in H as H2.
+    assumption.
+Qed.
+
+Lemma var_of_exp_binop_eq (e1 e2: exp) (b: binop):
+  var_of_exp (EBinop b e1 e2) = (var_of_exp e1) ++ (var_of_exp e2).
+Proof.
+  unfold var_of_exp.
+  simpl.
+  rewrite var_of_exp_aux_eq.
+  reflexivity.
+Qed.
+
+Lemma exp_no_var_is_evaluable (e: exp) (h: history):
+  var_of_exp e = [] ->
+  is_evaluable e h.
+Proof.
+  intros H.
+  induction e as [ c | b | (b, t) | op e1 IH1 e2 IH2 ].
+  - exists (VConst c).
+    reflexivity.
+  - exists (VInput b).
+    reflexivity.
+  - unfold var_of_exp in H.
+    discriminate.
+  - apply var_of_exp_binop_empty in H as [ H1 H2 ].
+    specialize (IH1 H1) as [ v1 Hv1 ].
+    specialize (IH2 H2) as [ v2 Hv2 ].
+    exists (VBinop op v1 v2).
+    simpl.
+    rewrite Hv1.
+    rewrite Hv2.
+    reflexivity.
+Qed.
+
+Lemma exp_with_evaluable_vars_is_evaluable (e: exp) (h: history):
+  Forall (fun v => Dict.is_in v h) (var_of_exp e) ->
+  exists v: value, eval_exp e h = Some v.
+Proof.
+  intros H.
+  induction e as [ c | b | (b, t) | op e1 IH1 e2 IH2 ].
+  - exists (VConst c).
+    reflexivity.
+  - exists (VInput b).
+    reflexivity.
+  - apply Forall_inv in H.
+    destruct H as [ v Hv ].
+    exists v.
+    assumption.
+  - rewrite var_of_exp_binop_eq in H.
+    apply Forall_app in H as [ H1 H2 ].
+    specialize (IH1 H1) as [ v1 Hv1 ].
+    specialize (IH2 H2) as [ v2 Hv2 ].
+    exists (VBinop op v1 v2).
+    simpl.
+    rewrite Hv1, Hv2.
+    reflexivity.
+Qed.
+
+Lemma exp_evaluable_have_evaluable_vars (e: exp) (h: history) (v: value):
+  eval_exp e h = Some v ->
+  Forall (fun v => Dict.is_in v h) (var_of_exp e).
+Proof.
+  intros H.
+  revert v H.
+  induction e as [ c' | | (b, t) | op e1 IH1 e2 IH2 ]; intros c H.
+  - constructor.
+  - constructor.
+  - constructor; [ | constructor ].
+    simpl in H.
+    exists c.
+    assumption.
+  - simpl in H.
+    destruct (eval_exp e1 h) as [ v1 | ]; [ | discriminate ].
+    destruct (eval_exp e2 h) as [ v2 | ]; [ | discriminate ].
+    specialize (IH1 v1 eq_refl).
+    specialize (IH2 v2 eq_refl).
+    rewrite var_of_exp_binop_eq.
+    apply Forall_app.
+    split; assumption.
+Qed.
+
+Theorem sem_eval_exp (e: exp) (h: history) (v: value):
+  eval_exp e h = Some v <-> sem_exp h e v.
+Proof.
+  split.
+  - intros H.
+    revert v H.
+    induction e as [ c' | t | (v, t) | op e1 IH1 e2 IH2 ]; intros c H.
+    + inversion H.
+      apply SeConst.
+    + inversion H.
+      subst.
+      apply SeInput.
+    + inversion H.
+      apply SeVar.
+      assumption.
+    + simpl in H.
+      destruct (eval_exp e1 h) as [ v1 | ]; [ | discriminate ].
+      destruct (eval_exp e2 h) as [ v2 | ]; [ | discriminate ].
+      specialize (IH1 v1 eq_refl).
+      specialize (IH2 v2 eq_refl).
+      inversion H.
+      apply SeBinop; assumption.
+  - intros H.
+    revert v H.
+    induction e as [ c' | t | (v, t) | op e1 IH1 e2 IH2 ]; intros c H.
+    + inversion H.
+      reflexivity.
+    + inversion H.
+      subst.
+      reflexivity.
+    + inversion H; subst.
+      simpl.
+      assumption.
+    + inversion H.
+      subst.
+      simpl.
+      specialize (IH1 v1 H5).
+      specialize (IH2 v2 H6).
+      rewrite IH1, IH2.
+      reflexivity.
+Qed.
