theories/Translations/LustreOrderedToImp.v
@@ -62,3 +62,356 @@ Definition tranlsate_lustre_node (n: Source.node): Target.method := {|
 
 Definition translate_node (n: LustreOrdered.node_ordered): Target.method :=
   tranlsate_lustre_node (LustreOrdered.node_ordered_is_node n).
+
+
+(** Lemmas *)
+
+Lemma correctness_exp (e: Source.exp) (h: Source.history) (out: Source.value):
+  Source.sem_exp h e out ->
+    Target.sem_exp (translate_history h) (translate_exp e) (translate_value out).
+Proof.
+  induction 1.
+
+  - (* EConst *)
+    apply Target.SeConst.
+
+  - (* EInput *)
+    apply Target.SeInput.
+
+  - (* EVar *)
+    apply Target.SeVar; simpl.
+
+    pose (fun e => translate_const (Stream.hd e)) as f.
+    now apply Dict.maps_to_map.
+
+  - (* EAnd *)
+    simpl.
+
+    apply Target.SeBinop.
+    + apply IHsem_exp1.
+    + apply IHsem_exp2.
+Qed.
+
+Lemma sem_exp_without_useless_var (e: Source.exp) (h: Source.history) (name: ident) (v: Source.value):
+  Source.sem_exp h e v ->
+  ~ In name (Source.var_of_exp e) ->
+    Source.sem_exp (Dict.remove name h) e v.
+Proof.
+  intros Hexp Hnin.
+  revert v Hexp.
+  induction e as [ c | t | [ b t ] | op e1 IH1 e2 IH2 ]; intros v Hexp.
+  - inversion Hexp.
+    subst.
+    apply Source.SeConst.
+  - inversion Hexp.
+    subst.
+    apply Source.SeInput.
+  - inversion Hexp.
+    subst.
+    unfold Source.var_of_exp in Hnin.
+    simpl in Hnin.
+    apply Source.SeVar.
+    simpl.
+    apply Dict.maps_to_not_removed; [ assumption | ].
+    intros Heq.
+    apply Hnin.
+    left.
+    assumption.
+  - inversion Hexp.
+    subst.
+    apply Source.SeBinop.
+    + apply IH1; [ | assumption ].
+      pose proof (Source.var_of_exp_not_in_binop e1 e2 name op) as [ H _ ]; assumption.
+    + apply IH2; [ | assumption ].
+      pose proof (Source.var_of_exp_not_in_binop e1 e2 name op) as [ _ H ]; assumption.
+Qed.
+
+Definition evaluable_equations (s: Target.stack) (l: list Source.equation): Prop :=
+  Forall (fun eq => exists v: Target.value, Target.sem_exp s (translate_exp (snd eq)) v) l.
+
+Lemma Forall_impl_in {A: Type} (P Q: A -> Prop) (l: list A):
+  (forall a : A, In a l -> P a -> Q a) ->
+  Forall P l -> Forall Q l.
+Proof.
+  intros H Hforall.
+  induction l as [ | x l ]; [ constructor | ].
+  constructor.
+  - apply H.
+    + left.
+      reflexivity.
+    + apply Forall_inv with (l := l).
+      assumption.
+  - apply IHl.
+    + intros a Hin HPa.
+      apply H; [ | assumption ].
+      right.
+      assumption.
+    + apply Forall_inv_tail with (a := x).
+      assumption.
+Qed.
+
+Lemma ordered_equations_are_evaluable (h: Source.history) (l: list Source.equation):
+  (Forall (fun eq =>
+      exists (v': Source.value),
+      Dict.maps_to (fst eq) v' h /\ Source.sem_exp h (snd eq) v'
+    ) l
+  ) ->
+  Ordered.t (LustreOrdered.equations_to_dag l) -> evaluable_equations (translate_history h) l.
+Proof.
+  intros Hhist Hord.
+  remember (LustreOrdered.equations_to_dag l) as dag.
+  revert l Hhist Heqdag.
+  induction Hord as [ | x l' | x lx l' ]; intros l Hhist Heqdag.
+  - symmetry in Heqdag.
+    apply LustreOrdered.dag_nil in Heqdag.
+    rewrite Heqdag.
+    constructor.
+  - destruct l as [ | eq l ]; [ constructor | ].
+    simpl in Heqdag.
+    destruct eq as [ eq_left eq_right ].
+    inversion Heqdag.
+    subst.
+    symmetry in H2.
+    apply Source.exp_no_var_is_evaluable with (h := h) in H2 as [ c Hc ].
+    constructor.
+    + exists (translate_value c).
+      apply correctness_exp.
+      apply Source.sem_eval_exp.
+      assumption.
+    + apply Forall_inv_tail in Hhist.
+      apply Forall_impl with (P := fun eq => exists v', Dict.maps_to (fst eq) v' h /\ Source.sem_exp h (snd eq) v'); [ | assumption ].
+      intros (name, exp) [ v' [ Hmaps Hsem ] ].
+      exists (translate_value v').
+      apply correctness_exp.
+      assumption.
+  - destruct l as [ | eq l ]; [ constructor | ].
+    simpl in Heqdag.
+    destruct eq as [ eq_left eq_right ].
+    inversion Heqdag.
+    subst.
+    constructor.
+    + assert (Forall (fun v => Dict.is_in v h) (Source.var_of_exp eq_right)) as Hvars.
+      * apply Forall_impl_in with (P := fun y => exists ly, In (y, ly) (LustreOrdered.equations_to_dag l)); [ | assumption ].
+        intros name Hin [ vars Hvars ].
+        apply Forall_inv in Hhist as [ v' [ Hmaps Hsem ] ].
+        apply Source.sem_eval_exp in Hsem.
+        pose proof (Source.exp_evaluable_have_evaluable_vars _ _ _ Hsem) as H'.
+        apply Forall_forall with (x := name) in H'; assumption.
+      * pose proof (Source.exp_with_evaluable_vars_is_evaluable _ _ Hvars) as [ c Hc ].
+        exists (translate_value c).
+        apply correctness_exp.
+        apply Source.sem_eval_exp.
+        assumption.
+    + apply Forall_inv_tail in Hhist.
+      apply Forall_impl with (P := fun eq => exists v', Dict.maps_to (fst eq) v' h /\ Source.sem_exp h (snd eq) v'); [ | assumption ].
+      intros (name, exp) [ v' [ Hmaps Hsem ] ].
+      exists (translate_value v').
+      apply correctness_exp.
+      assumption.
+Qed.
+
+Lemma translation_ordered_body (body: list Source.equation) (h: Source.history):
+  Ordered.t (LustreOrdered.equations_to_dag body) ->
+  (Forall (fun eq =>
+      exists (v': Source.value),
+      Dict.maps_to (fst eq) v' h /\ Source.sem_exp h (snd eq) v'
+  ) body ) ->
+  Forall (fun '(name, exp) => exists (v: Target.value), Target.sem_exp (translate_history h) (translate_exp exp) v) body.
+Proof.
+  intros H Hhist.
+  induction body; [ constructor | ].
+  constructor.
+  - destruct a.
+    apply ordered_equations_are_evaluable with (h := h) in H; [ | assumption ].
+    apply Forall_inv in H.
+    destruct H as [ c Hc ].
+    simpl in *.
+    exists c.
+    assumption.
+  - destruct a.
+    simpl in H.
+    apply IHbody.
+    + apply Ordered.cons in H.
+      assumption.
+    + apply Forall_inv_tail in Hhist.
+      assumption.
+Qed.
+
+Lemma translation_history_element_removal (h: Source.history) (name: ident):
+  Dict.remove name (translate_history h) = translate_history (Dict.remove name h).
+Proof.
+  apply Dict.equivalence_is_eq.
+  destruct h as [ l Hsort ].
+  split.
+  - intros i x H.
+    unfold Dict.map, Dict.maps_to, Dict.remove, Dict.find in *.
+    simpl in *.
+    induction l as [ | (j, y) l IH ]; [ discriminate | ].
+    simpl in *.
+    destruct (name =? j) eqn: Heq.
+    + apply PeanoNat.Nat.eqb_eq in Heq.
+      subst.
+      assumption.
+    + apply PeanoNat.Nat.eqb_neq in Heq.
+      simpl in *.
+      destruct (i =? j) eqn: Heq'; [ assumption | ].
+      apply IH.
+      * apply Sorted.cons in Hsort.
+        assumption.
+      * apply PeanoNat.Nat.eqb_neq in Heq'.
+        assumption.
+  - intros i x H.
+    unfold Dict.map, Dict.maps_to, Dict.remove, Dict.find in *.
+    simpl in *.
+    induction l as [ | (j, y) l IH ]; [ discriminate | ].
+    simpl in *.
+    destruct (name =? j) eqn: Heq.
+    + apply PeanoNat.Nat.eqb_eq in Heq.
+      subst.
+      assumption.
+    + apply PeanoNat.Nat.eqb_neq in Heq.
+      simpl in *.
+      destruct (i =? j) eqn: Heq'; [ assumption | ].
+      apply IH.
+      * apply Sorted.cons in Hsort.
+        assumption.
+      * apply PeanoNat.Nat.eqb_neq in Heq'.
+        assumption.
+Qed.
+
+Lemma correctness_translation_equation (h: Source.history) (name: ident) (exp: Source.exp) (v: Source.value):
+  Source.sem_exp h exp v ->
+  Dict.maps_to name v h ->
+  ~ In name (Source.var_of_exp exp) ->
+  Target.sem_stmt (translate_history (Dict.remove name h)) (translate_equation (name, exp)) (translate_history h).
+Proof.
+  intros Hexp Hmaps Hnin.
+  unfold translate_equation.
+  simpl.
+  rewrite Dict.remove_then_add_same_elt with (i := name) (x := translate_value v).
+  - rewrite translation_history_element_removal.
+    apply Target.SeAssign.
+    apply correctness_exp.
+    apply sem_exp_without_useless_var; assumption.
+  - apply Dict.maps_to_map.
+    assumption.
+Qed.
+
+Theorem correctness_node (n: LustreOrdered.node_ordered) (m: Target.method) (h: Source.history) (v: Stream.t Source.const):
+  (forall (i: ident), Dict.is_in i h <-> In i (map fst (Source.n_body (LustreOrdered.node_ordered_is_node n)))) ->
+  (Forall (fun eq =>
+      exists (v': Source.value),
+      Dict.maps_to (fst eq) v' h /\ Source.sem_exp h (snd eq) v'
+    ) (Source.n_body (LustreOrdered.node_ordered_is_node n))
+  ) ->
+    Target.sem_stmt (Dict.empty _) (Target.m_body (translate_node n)) (translate_history h).
+Proof.
+  intros Hhist Hsource.
+  destruct n.
+  destruct node_ordered_is_node.
+  simpl in *.
+  clear n_assigned_out n_inputs_equations n_no_einputs_in_other.
+  revert h Hhist Hsource.
+  induction n_body as [ | (eq_left, eq_right) n_body IH ]; intros h Hhist Hsource.
+  - simpl.
+
+    assert (h = Dict.empty _).
+    { apply Dict.no_element_is_empty.
+      destruct h as [ h_elements Hsort ].
+      simpl.
+      destruct h_elements as [ | (i, x) h_elements ]; [ reflexivity | ].
+      exfalso.
+      apply Hhist with (i := i).
+      exists x.
+      unfold Dict.maps_to, Dict.find.
+      simpl.
+      rewrite PeanoNat.Nat.eqb_refl.
+      reflexivity. }
+
+    subst.
+    unfold translate_node_body; simpl.
+    apply Target.SeNop.
+  - apply Ordered.cons in ordered as H.
+    apply Ordered.cons in ordered as ordered_inner_body.
+    fold LustreOrdered.equations_to_dag in ordered_inner_body.
+    apply translation_ordered_body with (h := h) in ordered as Htrans; [ | assumption ].
+
+    assert (incl (map fst n_body) (map fst n_vars)) as Hincl.
+    { intros x Hx.
+      apply n_assigned_vars_are_vars.
+      right.
+      assumption. }
+
+    apply Forall_inv_tail in Hsource as Hsource_tail.
+
+    pose (Dict.remove eq_left h) as hprev.
+    pose proof (IH Hincl ordered_inner_body hprev) as IHprev.
+    unfold translate_node_body.
+    simpl.
+    apply Forall_inv in Hsource.
+    destruct Hsource as [ v' [ Hv'1 Hv'2 ] ].
+    apply Forall_inv in Htrans as [ w Hw ].
+    apply Target.SeSeq with (s2 := translate_history hprev).
+    2: { unfold translate_equation, hprev.
+      simpl.
+      apply correctness_translation_equation with (v := v'); [ assumption | assumption | ].
+      apply Ordered.var_not_need_itself in ordered.
+      assumption. }
+
+    apply IHprev.
+    * intros i.
+      split.
+      -- intros [ x Hix ].
+         unfold hprev in Hix.
+         apply Dict.maps_to_with_removal in Hix as Hih.
+         apply Dict.maps_to_imp_is_in in Hih.
+         specialize (Hhist i) as Hi.
+         destruct Hi as [ Hi1 Hi2].
+         specialize (Hi1 Hih) as [ Heq | Hin ]; [ | assumption ].
+         exfalso.
+         simpl in Heq.
+         subst.
+         apply Dict.removed_element_not_in with (i := i) (d := h).
+         exists x.
+         assumption.
+      -- intros Hi.
+         specialize (Hhist i) as Hhisti.
+         destruct Hhisti as [ Hi1 Hi2].
+         unfold hprev.
+         destruct (PeanoNat.Nat.eq_dec i eq_left).
+         ++ subst.
+            exfalso.
+            apply Ordered.vars_no_dups in ordered.
+            apply ordered.
+            rewrite <- LustreOrdered.dag_names.
+            assumption.
+         ++ specialize (Hi2 (in_cons _ _ _ Hi)).
+            destruct Hi2 as [ x Hx ].
+            apply Dict.maps_to_not_removed with (j := eq_left) in Hx; [ | assumption ].
+            exists x.
+            assumption.
+    * apply Forall_forall.
+      intros (i, x) Hin.
+      apply Forall_forall with (x := (i, x)) in Hsource_tail as Hix; [ | assumption ].
+      destruct Hix as [ w' [ Hw'1 Hw'2 ] ].
+      exists w'.
+      split.
+      -- simpl in *.
+         unfold hprev.
+         destruct (PeanoNat.Nat.eq_dec i eq_left).
+         ++ subst.
+            exfalso.
+            apply Ordered.vars_no_dups in ordered.
+            apply ordered.
+            rewrite <- LustreOrdered.dag_names.
+            apply in_map with (f := fst) in Hin.
+            assumption.
+         ++ apply Dict.maps_to_not_removed; assumption.
+      -- simpl in *.
+         unfold hprev.
+         apply sem_exp_without_useless_var; [ assumption | ].
+         apply Ordered.vars_coherence with (l := LustreOrdered.equations_to_dag n_body) (y := i) (lx := Source.var_of_exp eq_right); [ assumption | ].
+         apply in_map with (f := fun '(i, x) => (i, Source.var_of_exp x)) in Hin.
+         rewrite LustreOrdered.equations_to_dag_is_map.
+         assumption.
+Qed.
