theories/Base.v
@@ -4,8 +4,6 @@ From Coq Require Export List Nat String.
 From Coq Require Export Lia.
 
 Export ListNotations.
-
-Open Scope string_scope.
 Open Scope nat_scope.
 
 
