theories/Datatypes/Ordered.v
@@ -12,3 +12,81 @@ Inductive t {A: Type}: list (A * list A) -> Prop :=
       ~ In x (map fst l) ->
       (Forall (fun y => exists ly: list A, In (y, ly) l) lx) ->
       t ((x, lx) :: l).
+
+
+Lemma cons {A: Type} (l: list (A * list A)) (x: A * list A):
+  t (x :: l) -> t l.
+Proof.
+  intros H.
+  inversion H; subst.
+  - assumption.
+  - assumption.
+Qed.
+
+Lemma vars_no_dups {A: Type} (l: list (A * list A)) (x: A) (lx: list A):
+  t ((x, lx) :: l) ->
+  ~ In x (map fst l).
+Proof.
+  intros Hord Hin.
+  inversion Hord; subst; auto.
+Qed.
+
+Lemma var_cons_in_right_side {A: Type} (x y: A) (lx: list A) (l: list (A * list A)):
+  t ((x, lx) :: l) ->
+  In y lx ->
+  exists ly: list A, In (y, ly) l.
+Proof.
+  intros Hord Hin.
+  inversion Hord; subst.
+  - inversion Hin.
+  - apply Forall_forall with (x := y) in H4; assumption.
+Qed.
+
+Lemma var_in_right_side {A: Type} (x y: A) (lx: list A) (l: list (A * list A)):
+  t l ->
+  In (x, lx) l ->
+  In y lx ->
+  exists ly: list A, In (y, ly) l.
+Proof.
+  intros Hord Hx Hy.
+  induction l as [ | (z, lz) l IH ]; [ inversion Hx | ].
+  destruct Hx as [ Heq | Hx ].
+  - inversion Heq.
+    subst.
+    apply var_cons_in_right_side with (y := y) in Hord; [ | assumption].
+    destruct Hord as [ ly Hly ].
+    exists ly.
+    right.
+    assumption.
+  - apply cons in Hord.
+    specialize (IH Hord Hx) as [ ly Hly ].
+    exists ly.
+    right.
+    assumption.
+Qed.
+
+Lemma vars_coherence {A: Type} (l: list (A * list A)) (x y: A) (lx ly: list A):
+  t ((x, lx) :: l) ->
+  In (y, ly) l ->
+  ~ In x ly.
+Proof.
+  intros Hord Hin Hnin.
+  apply cons in Hord as Hord_inner.
+  pose proof (var_in_right_side _ _ _ _ Hord_inner Hin Hnin) as [ lz Hlz ].
+  apply vars_no_dups in Hord.
+  apply Hord.
+  apply in_map with (f := fst) in Hlz.
+  assumption.
+Qed.
+
+Lemma var_not_need_itself {A: Type} (x: A) (lx: list A) (l: list (A * list A)):
+  t ((x, lx) :: l) ->
+  ~ In x lx.
+Proof.
+  intros Hord Hin.
+  pose proof (var_cons_in_right_side _ _ _ _ Hord Hin) as [ ly Hly ].
+  apply vars_no_dups in Hord.
+  apply Hord.
+  apply in_map with (f := fst) in Hly.
+  assumption.
+Qed.
