theories/Languages/LustreOrdered.v
@@ -17,3 +17,55 @@ Record node_ordered := mk_node_ordered {
   node_ordered_is_node :> Lustre.node;
   ordered: Ordered.t (equations_to_dag (Lustre.n_body node_ordered_is_node));
 }.
+
+
+(** Lemmas *)
+
+Lemma dag_names (equations: list Lustre.equation):
+  map fst equations = map fst (equations_to_dag equations).
+Proof.
+  induction equations.
+  - reflexivity.
+  - destruct a.
+    simpl.
+    rewrite IHequations.
+    reflexivity.
+Qed.
+
+Lemma dag_length (equations: list Lustre.equation):
+  List.length equations = List.length (equations_to_dag equations).
+Proof.
+  induction equations.
+  - simpl.
+    reflexivity.
+  - destruct a.
+    simpl.
+    apply f_equal.
+    assumption.
+Qed.
+
+Lemma dag_nil (equations: list Lustre.equation):
+  equations = [] <-> equations_to_dag equations = [].
+Proof.
+  split.
+  - intros eq.
+    pose proof (@f_equal _ _ (@List.length Lustre.equation) _ _ eq) as H.
+    simpl in H.
+    rewrite dag_length in H.
+    apply length_zero_iff_nil.
+    assumption.
+  - intros eq.
+    pose proof (@f_equal _ _ (@List.length _) _ _ eq) as H.
+    rewrite <- dag_length in H.
+    apply length_zero_iff_nil.
+    assumption.
+Qed.
+
+Lemma equations_to_dag_is_map (equations: list Lustre.equation):
+  equations_to_dag equations = map (fun '(name, exp) => (name, Lustre.var_of_exp exp)) equations.
+Proof.
+  induction equations as [ | (name, exp) l IH ]; [ reflexivity | ].
+  simpl.
+  f_equal.
+  assumption.
+Qed.
